Logic/Modal/Standard/Kripke/Reducible.lean
@@ -5,39 +5,40 @@ namespace LO.Modal.Standard
 
 namespace Kripke
 
-variable {W α : Type*} [DecidableEq α]
-variable {Λ₁ Λ₂ : AxiomSet α} {P₁ P₂ : Frame W α → Prop}
-variable [hSound₁ : Sound Λ₁ 𝔽(Λ₁, W)] [hSound₂ : Sound Λ₂ 𝔽(Λ₂, W)]
-variable [hComp₁ : Complete Λ₁ 𝔽(Λ₁, W)] [hComp₂ : Complete Λ₂ 𝔽(Λ₂, W)]
-variable (hDec₁ : AxiomSetDefinability W Λ₁ P₁) (hDec₂ : AxiomSetDefinability W Λ₂ P₂)
+variable {W : Type*} {α : Type u} [DecidableEq α]
+variable {Λ₁ Λ₂ : AxiomSet α} {P₁ P₂ : ∀ {W : Type u}, [Inhabited W] → Frame W α → Prop}
+variable [hSound₁ : Sound Λ₁ 𝔽(Λ₁)] [hSound₂ : Sound Λ₂ 𝔽(Λ₂)]
+variable [hComp₁ : Complete Λ₁ 𝔽(Λ₁)] [hComp₂ : Complete Λ₂ 𝔽(Λ₂)]
+variable (hDef₁ : AxiomSetDefinability Λ₁ P₁) (hDef₂ : AxiomSetDefinability Λ₂ P₂)
 
-lemma reducible_of_subset_axiomSetFrameClass (hs : 𝔽(Λ₂, W) ⊆ 𝔽(Λ₁, W)) : Λ₁ ≤ₛ Λ₂ := by
+lemma reducible_of_subset_axiomSetFrameClass (hs : ∀ {W}, [hiW : Inhabited W] → ∀ {F}, 𝔽(Λ₂) W hiW F → 𝔽(Λ₁) W hiW F) : Λ₁ ≤ₛ Λ₂ := by
   apply System.reducible_iff.mpr;
   intro p hp;
   apply hComp₂.complete;
-  intro F hF;
-  exact hSound₁.sound hp F (hs hF);
+  intro W _ F hF;
+  exact hSound₁.sound hp W F $ hs hF;
 
-lemma reducible_of_definability (hs : ∀ {F : Frame W α}, P₂ F → P₁ F) : Λ₁ ≤ₛ Λ₂ := by
-  apply reducible_of_subset_axiomSetFrameClass (W := W);
-  intro h hF;
-  apply iff_definability_memAxiomSetFrameClass hDec₁ |>.mp;
-  exact hs $ iff_definability_memAxiomSetFrameClass hDec₂ |>.mpr hF;
+lemma reducible_of_definability (hs : ∀ {W}, [Inhabited W] → ∀ {F : Frame W α}, P₂ F → P₁ F) : Λ₁ ≤ₛ Λ₂ := by
+  apply reducible_of_subset_axiomSetFrameClass;
+  intro W hiW F hF;
+  apply iff_definability_memAxiomSetFrameClass hDef₁ |>.mpr;
+  exact hs $ iff_definability_memAxiomSetFrameClass hDef₂ |>.mp hF;
 
-lemma equiv_of_eq_axiomSetFrameClass (heq : 𝔽(Λ₁, W) = 𝔽(Λ₂, W)) : Λ₁ =ₛ Λ₂ := by
+lemma equiv_of_eq_axiomSetFrameClass
+  (hs₁ : ∀ {W}, [hiW : Inhabited W] → ∀ {F}, 𝔽(Λ₂) W hiW F → 𝔽(Λ₁) W hiW F)
+  (hs₂ : ∀ {W}, [hiW : Inhabited W] → ∀ {F}, 𝔽(Λ₁) W hiW F → 𝔽(Λ₂) W hiW F)
+  : Λ₁ =ₛ Λ₂ := by
   apply System.Equiv.antisymm_iff.mpr;
   constructor;
-  . exact reducible_of_subset_axiomSetFrameClass heq.symm.subset;
-  . exact reducible_of_subset_axiomSetFrameClass heq.subset;
+  . apply reducible_of_subset_axiomSetFrameClass hs₁;
+  . apply reducible_of_subset_axiomSetFrameClass hs₂;
 
-lemma equiv_of_iff_definability (h : ∀ {F : Frame W α}, P₁ F ↔ P₂ F) : Λ₁ =ₛ Λ₂ := by
+lemma equiv_of_iff_definability (h : ∀ {W}, [Inhabited W] → ∀ {F : Frame W α}, P₁ F ↔ P₂ F) : Λ₁ =ₛ Λ₂ := by
   apply System.Equiv.antisymm_iff.mpr;
   constructor;
-  . apply reducible_of_definability hDec₁ hDec₂;
-    intro F hF;
-    exact h.mpr hF;
-  . apply reducible_of_definability hDec₂ hDec₁;
-    intro F hF;
-    exact h.mp hF;
+  . apply reducible_of_definability hDef₁ hDef₂;
+    intros; apply h.mpr; assumption;
+  . apply reducible_of_definability hDef₂ hDef₁;
+    intros; apply h.mp; assumption;
 
 end LO.Modal.Standard.Kripke
